proved inv5

Isabelle2/R3_Refines_R1.thy
@@ -6,8 +6,8 @@ begin
 
 section {* A few lemmas *}
 
-locale receive_1b_lemmas = receive_1b votes as log for votes as log +
-  assumes votes_default:"\<And> a . finfun_default (votes $ a) = None"
+locale receive_1b_lemmas = receive_1b onebs as log for onebs as log +
+  assumes votes_default:"\<And> a . finfun_default (onebs $ a) = None"
     and log_default:"finfun_default log = amp_r3.inst_status.Free" and fin:"finite as"
 begin
 
@@ -69,8 +69,9 @@ locale ref_proof_4 = quorums quorums + amp_r3 leader next_bal as quorums
     and ampr1_ioa :: "(('v, 'a, 'l) ampr1_state, 'v paxos_action) ioa" 
   defines "ampr3_ioa \<equiv> ioa" and "ampr1_ioa \<equiv> r1.ioa"
   fixes a1 a2 a3
-  assumes "a1 \<in> as" and "a2 \<in> as" and "a3 \<in> as" and "a1 \<noteq> a2" and "a3 \<noteq> a2" and "a3 \<noteq> a1"
-  (* assumes a_inf:"\<not> finite (UNIV::'a set)" *)
+  assumes at_least_3:"a1 \<in> as \<and> a2 \<in> as \<and> a3 \<in> as \<and> a1 \<noteq> a2 \<and> a3 \<noteq> a2 \<and> a3 \<noteq> a1"
+  assumes fin:"finite as" and infin:"infinite (UNIV::'a set)"
+    -- {* @{term "UNIV::'a set"} must be infinite for @{term finfun_default} to make sense. *}
 begin
 
 interpretation IOA .
@@ -85,19 +86,20 @@ lemmas init_defs = ampr3_ioa_def ioa_def global_start_def local_start_def
 method trans_cases =
   (simp add:is_trans_def ampr3_ioa_def ioa_def, elim trans_cases)
 
-definition inv1 where inv1_def[inv_proofs_defs]:"inv1 s \<equiv> \<forall> a . acceptors (lstate s a) = as \<and> id (lstate s a) = a"
+definition inv1 where inv1_def[inv_proofs_defs]:
+  "inv1 s \<equiv> \<forall> a . acceptors (lstate s a) = as \<and> id (lstate s a) = a"
 lemma inv1:"invariant ampr3_ioa inv1"
   apply (rule invariantI)
    apply (simp add:inv1_def init_defs)
   apply (rm_reachable)
   apply trans_cases
-         apply (auto simp add:Let_def inv1_def action_defs)
+         apply (auto simp add:inv1_def action_defs)
   done
 declare inv1[invs]
 
 definition inv2 where inv2_def:
   "inv2 s \<equiv> \<forall> i b v a . Packet a (Phase2a i b v) \<in> network s 
-    \<longrightarrow> log (lstate s (leader b)) $ i = Free"
+    \<longrightarrow> log (lstate s (leader b)) $ i = Free" (* What? *)
 lemma inv2:"invariant ampr3_ioa inv2"
   apply (rule invariantI)
    apply (simp add:inv2_def init_defs)
@@ -111,7 +113,7 @@ lemma inv2:"invariant ampr3_ioa inv2"
 definition inv3 where 
   "inv3 s \<equiv> \<forall> i a b d1 v1 d2 v2 . 
     Packet d1 (Phase2b a i b v1) \<in> network s \<and> Packet d2 (Phase2b a i b v2) \<in> network s
-    \<longrightarrow> v1 = v2 \<and> d1 = d2"
+    \<longrightarrow> v1 = v2 \<and> d1 = d2 \<and> d1 = leader b"
 lemma inv2:"invariant ampr3_ioa inv2"
   apply (rule invariantI)
    apply (simp add:inv2_def init_defs)
@@ -121,7 +123,66 @@ lemma inv2:"invariant ampr3_ioa inv2"
   apply trans_cases
   oops
 
-definition inv4 where "inv4 s \<equiv> 
+definition inv5 :: "('a,'v)global_state \<Rightarrow> bool" where inv5_def[inv_proofs_defs]:
+  "inv5 s \<equiv> \<forall> a b a2 p . 
+    finfun_default ((acc.onebs (lstate s a)) $ b $ a2) = None
+    \<and> (finfun_default (acc.votes (lstate s a)) = None)
+    \<and> (p \<in> network s \<longrightarrow> 
+        (case p of Packet _ (Phase1b _ _ vs) \<Rightarrow> finfun_default vs = None
+        | Packet _ _ \<Rightarrow> True))"
+lemma inv5:"invariant ampr3_ioa inv5"
+  apply (rule invariantI)
+   apply (simp add:inv5_def init_defs finfun_default_const)
+  apply (insert invs)
+  apply (instantiate_invs)
+  apply (rm_reachable)
+  apply (trans_cases;
+    (simp add:inv1_def inv5_def action_defs finfun_default_update_const split!:packet.splits msg.splits; fail)?)
+  subgoal premises prems for s t act a b vs m p a2 (* receive_1b*)
+  proof -
+    have 1:"acc.onebs (lstate t a) = new_onebs (acc.onebs (lstate s a)) vs b a2"
+      using prems(2,5,6) by (auto simp add:inv1_def action_defs)
+    show ?thesis
+    proof (auto simp add:inv5_def)
+      fix a' b' a2'
+      show "finfun_default (acc.onebs (lstate t a') $ b' $ a2') = None" 
+      proof (cases "a' = a")
+        case True
+        have 2:"acc.onebs (lstate t a') = new_onebs (acc.onebs (lstate s a')) vs b a2"
+          using 1 True by auto
+        have 3:"finfun_default (acc.onebs (lstate s a') $ b' $ a2') = None"
+          using prems(1) by (auto simp add:inv5_def)
+        show ?thesis using 2 3 prems(1,4,7)
+          apply (auto simp add: inv5_def new_onebs_def update_onebs.new_onebs_def)
+          apply (case_tac "b' = b", case_tac "a2' = a2") apply auto
+          by fastforce
+      next
+        case False
+        then show ?thesis using prems(1,6) by (simp add:inv5_def) 
+      qed
+    next
+      fix a
+      show "finfun_default (votes (lstate t a)) = None" using prems 
+        by (simp add:inv1_def inv5_def action_defs finfun_default_update_const split!:packet.splits msg.splits)
+    next 
+      fix p
+      let ?sa = "lstate s a"
+      have 1:"let msgs = msgs (acc.onebs ?sa $ b) (acc.acceptors ?sa) (log ?sa)
+        in snd (receive_1b ?sa a2 b vs) \<subseteq> \<Union> {send_all ?sa m | m . m \<in> msgs} "
+        by (auto simp add:inv1_def action_defs)
+      have 2:"\<And> m . let msgs = msgs (acc.onebs ?sa $ b) (acc.acceptors ?sa) (log ?sa) in 
+        m \<in> \<Union> {send_all ?sa m | m . m \<in> msgs} \<Longrightarrow> case m of Packet _ (Phase2a _ _ _) \<Rightarrow> True | _ \<Rightarrow> False"
+        using r1.msgs_lemma by (fastforce simp add:send_all_def)
+      from 1 2 have "\<And> p . p \<in> snd (receive_1b ?sa a2 b vs) \<Longrightarrow> 
+        case p of Packet _ (Phase2a _ _ _) \<Rightarrow> True | _ \<Rightarrow> False" by auto
+      moreover have "network t = snd (receive_1b ?sa a2 b vs) \<union> network s" using prems(5,6) by auto
+      ultimately show "p \<in> network t \<Longrightarrow> case p of Packet _ (Phase1b _ _ vs) \<Rightarrow> finfun_default vs = None | Packet _ _ \<Rightarrow> True"  
+        using prems(1) by (force simp add:inv5_def inv1_def split!:packet.splits msg.splits)
+    qed
+  qed
+  done
+        
+definition inv4 where "inv4 s \<equiv>
   (\<forall> a . finfun_default (log (lstate s a)) = Free)"
   
 lemma inv4:"invariant ampr3_ioa inv4"
@@ -136,21 +197,19 @@ lemma inv4:"invariant ampr3_ioa inv4"
           amp_r3.next_inst_lemma
           split!:if_splits msg.splits packet.splits inst_status.splits) oops
 
-  
-  
 fun extract_vs where 
   "extract_vs (Fwd v) = {v}"
 | "extract_vs (Phase2a _ _ v) = {v}"
 | "extract_vs (Phase2b _ _ _ v) = {v}"
 | "extract_vs (Phase1b _ _ ff) = {v . \<exists> i b . ff $ i = Some (v,b)}"
-  -- {* Could be @{term "{ff $ i \<bind> (Some o fst) | i . True} \<bind> option_as_set" }*}
+  -- {* Could be @{term "{ff $ i \<bind> (Some o fst) | i . True} \<bind> option_as_set" } *}
 | "extract_vs _ = {}"
   
 definition propCmd where "propCmd s \<equiv> \<Union> ((\<lambda> p . case p of Packet _ m \<Rightarrow> extract_vs m) ` network s)"
 
 definition ref_map where "ref_map s \<equiv> \<lparr>
   ampr1_state.propCmd = propCmd s,
-  ballot = \<lambda> a . local_state.ballot (lstate s a),
+  ballot = \<lambda> a . acc.ballot (lstate s a),
   vote = \<lambda> i a b . if (\<exists> a2 v . Packet a2 (Phase2b a i b v) \<in> network s) 
     then Some (the_elem {v . \<exists> a2 . Packet a2 (Phase2b a i b v) \<in> network s}) else None,
   suggestion = \<lambda> i b . if (\<exists> a v. Packet a (Phase2a i b v) \<in> network s) 
@@ -167,32 +226,26 @@ lemma "is_ref_map ref_map ampr3_ioa ampr1_ioa"
   apply (instantiate_invs)
   apply (rm_reachable)
   apply trans_cases
-  subgoal premises prems for s s' t act a v (* Propose *)
-  proof -
-    let ?ef = "[(act, s'\<lparr>ampr1_state.propCmd := insert v (ampr1_state.propCmd s')\<rparr>)]"
-    show ?thesis
-      apply (intro exI[where ?x="?ef"])
-      apply (intro conjI)
-        prefer 3
-        apply (force simp add:trace_match_def trace_def schedule_def externals_def
-          filter_act_def ampr1_ioa_def r1.ioa_def paxos_asig_def Let_def is_trans_def 
-          r1.trans_def split!:if_splits)
-       apply simp
-      subgoal proof (cases "leader (local_state.ballot (lstate s a)) = local_state.id (lstate s a)")
-        case False
-        with prems(1,4) show ?thesis by (simp add:propose_def send_all_def fwd_sim_def propCmd_def)
-      next
-        case True thm prems
-        have 1:"\<And> a . local_state.ballot (lstate t a) = ballot s' a" using prems(1,4) True 
-          by (simp add:do_2a_def propose_def send_all_def fwd_sim_def Let_def propCmd_def)
-        have 2:"network t = network s \<union> {Packet a2 (Phase2a (next_inst (lstate s a)) (local_state.ballot (lstate s a)) v) 
-            | a2 . a2 \<noteq> a \<and> a2 \<in> acceptors (lstate s a)}"
-          using prems(4,2) True
-          by (fastforce simp add:do_2a_def propose_def send_all_def fwd_sim_def propCmd_def Let_def inv1_def)
-        show ?thesis using 1 2 prems(1,2) apply (auto simp add:sim_defs inv1_def split!:msg.splits packet.splits)
-              apply (metis ref_proof_3.axioms(2) ref_proof_3_axioms ref_proof_3_axioms_def)
-             apply meson defer
-          apply meson oops
+  subgoal premises prems for s t act a v (* Propose *)
+  proof (intro exI[where ?x="ref_map s"] exI[where ?x="[(act, ref_map t)]"])
+    thm prems
+    have "ref_map t = (ref_map s)\<lparr>propCmd := insert v (ampr1_state.propCmd (ref_map s))\<rparr>"
+    proof (cases "leader (acc.ballot (lstate s a)) = a")
+      case True 
+      have 1:"network t = (network s \<union> (snd (do_2a (lstate s a) v)))" using prems(1) prems(3) True
+        by (simp add:inv1_def propose_def)
+      have 2:"\<And> a . acc.ballot (lstate s a) = acc.ballot (lstate t a)" using prems(1) prems(3) True
+        by (simp add:inv1_def propose_def do_2a_def Let_def)
+      show ?thesis using prems(1) 1 2 at_least_3 (* Note: does not hold if we have only one acceptor in the systems *)
+        apply (auto simp add:inv1_def ref_map_def action_defs propCmd_def fun_eq_iff split!:packet.splits msg.splits if_splits)
+           apply metis (* Here we need a lemma about all those the_elem terms. *)
+        sorry
+    next
+      case False
+      then show ?thesis using prems(1) prems(3)
+        by (auto simp add:inv1_def ref_map_def action_defs propCmd_def fun_eq_iff split!:packet.splits msg.splits if_splits)
+    qed oops
+    
 end
 
 
@@ -246,9 +299,9 @@ lemma inv1:"invariant ghost_ioa inv1"
       apply(simp add:receive_2a_def Let_def send_all_def split:if_splits option.splits)
      apply(simp add:receive_2b_def Let_def send_all_def split:if_splits option.splits)
     apply(simp add:receive_1b_def receive_1b.msgs_def msgs_def Let_def send_all_def split:if_splits option.splits)
-  subgoal proof -
-    fix a :: "('a, 'v) global_state" and b :: "'v set" and ac :: 'a and bb :: nat and vs :: "nat \<Rightarrow>f ('v \<times> nat) option" and ad :: "('a, 'v) local_state" and bc :: "('a, 'v) packet set" and ae :: 'a and v :: 'v
-    assume a1: "(\<exists>x. finfun_dom (receive_1b.new_log (the (local_state.onebs (lstate a ac) $ bb)) (acceptors (lstate a ac)) (log (lstate a ac))) $ x \<and> (Fwd v::('a, 'v) msg) = (case the_elem (receive_1b.max_per_inst (the (local_state.onebs (lstate a ac) $ bb)) (acceptors (lstate a ac)) $ x) of (v, b) \<Rightarrow> Phase2a x b v)) \<and> ae \<in> acceptors (lstate a ac) \<and> ae \<noteq> local_state.id (lstate a ac)"
+  subgoal proof - oops
+    fix a :: "('a, 'v) global_state" and b :: "'v set" and ac :: 'a and bb :: nat and vs :: "nat \<Rightarrow>f ('v \<times> nat) option" and ad :: "('a, 'v) acc" and bc :: "('a, 'v) packet set" and ae :: 'a and v :: 'v
+    assume a1: "(\<exists>x. finfun_dom (receive_1b.new_log (the (acc.onebs (lstate a ac) $ bb)) (acceptors (lstate a ac)) (log (lstate a ac))) $ x \<and> (Fwd v::('a, 'v) msg) = (case the_elem (receive_1b.max_per_inst (the (acc.onebs (lstate a ac) $ bb)) (acceptors (lstate a ac)) $ x) of (v, b) \<Rightarrow> Phase2a x b v)) \<and> ae \<in> acceptors (lstate a ac) \<and> ae \<noteq> acc.id (lstate a ac)"
     have "\<And>n p v. (case p of (v, na) \<Rightarrow> Phase2a n na v) \<noteq> (Fwd v::('a, 'v) msg)"
       by (metis amp_r3.msg.distinct(17) case_prod_conv surj_pair)
     then show "v \<in> b"
@@ -281,12 +334,12 @@ definition update_hist where "update_hist s h a s' \<equiv> case a of
   | Internal \<Rightarrow> 
       h\<lparr>vote := \<lambda> i a b . case (votes (lstate s' a) $ i) of Some (v,b2) \<Rightarrow> 
           (if b = b2 then Some v else (vote h i a b)) | None \<Rightarrow> None,
-        ampr1_state.ballot := \<lambda> a . local_state.ballot (lstate s' a),
+        ampr1_state.ballot := \<lambda> a . acc.ballot (lstate s' a),
         suggestion := \<lambda> i b . case (log (lstate s' (leader b)) $ i) of Proposed v \<Rightarrow> (
               case (log (lstate s (leader b)) $ i) of Free \<Rightarrow> Some v | _ \<Rightarrow> suggestion h i b)
           | Decided v \<Rightarrow> suggestion h i b
           | Free \<Rightarrow> None,
-        onebs := \<lambda> a b . if local_state.ballot (lstate s' a) = b \<and> local_state.ballot (lstate s' a) \<noteq> b
+        onebs := \<lambda> a b . if acc.ballot (lstate s' a) = b \<and> acc.ballot (lstate s' a) \<noteq> b
           then Some (op$ (votes (lstate s a))) else None\<rparr>
   | _ \<Rightarrow> h"
 
@@ -320,11 +373,11 @@ lemma inv1:"invariant ghost_ioa inv1"
     apply (simp add:receive_2b_def Let_def send_all_def split:if_splits)
    apply (simp add:receive_1b_def Let_def send_all_def msgs_def receive_1b.msgs_def split:if_splits)
   subgoal proof -
-    fix a :: "('a, 'v) global_state" and b :: "('v, 'a, ?'l) ampr1_state" and ac :: 'a and bb :: nat and vs :: "nat \<Rightarrow>f ('v \<times> nat) option" and ad :: "('a, 'v) local_state" and bc :: "('a, 'v) packet set" and ae :: 'a and v :: 'v
-    assume a1: "(\<exists>x. finfun_dom (receive_1b.new_log (the (local_state.onebs (lstate a ac) $ bb)) (acceptors (lstate a ac)) (log (lstate a ac))) $ x \<and> (Fwd v::('a, 'v) msg) = (case the_elem (receive_1b.max_per_inst (the (local_state.onebs (lstate a ac) $ bb)) (acceptors (lstate a ac)) $ x) of (v, b) \<Rightarrow> Phase2a x b v)) \<and> ae \<in> acceptors (lstate a ac) \<and> ae \<noteq> local_state.id (lstate a ac)"
+    fix a :: "('a, 'v) global_state" and b :: "('v, 'a, ?'l) ampr1_state" and ac :: 'a and bb :: nat and vs :: "nat \<Rightarrow>f ('v \<times> nat) option" and ad :: "('a, 'v) acc" and bc :: "('a, 'v) packet set" and ae :: 'a and v :: 'v
+    assume a1: "(\<exists>x. finfun_dom (receive_1b.new_log (the (acc.onebs (lstate a ac) $ bb)) (acceptors (lstate a ac)) (log (lstate a ac))) $ x \<and> (Fwd v::('a, 'v) msg) = (case the_elem (receive_1b.max_per_inst (the (acc.onebs (lstate a ac) $ bb)) (acceptors (lstate a ac)) $ x) of (v, b) \<Rightarrow> Phase2a x b v)) \<and> ae \<in> acceptors (lstate a ac) \<and> ae \<noteq> acc.id (lstate a ac)"
     have "\<And>n p v. (case p of (v, na) \<Rightarrow> Phase2a n na v) \<noteq> (Fwd v::('a, 'v) msg)"
       by (metis amp_r3.msg.distinct(17) case_prod_conv surj_pair)
-    then show "v \<in> propCmd b"
+    then show "v \<in> propCmd b" oops
       using a1 by metis
   qed
   apply (simp add:receive_fwd_def do_2a_def Let_def send_all_def split:if_splits)
@@ -363,7 +416,7 @@ lemma "is_ref_map ref_map ghost_ioa ampr1_ioa"
      prefer 2
      apply (simp add:trace_match_def trace_def schedule_def externals_def
         filter_act_def ampr1_ioa_def r1.ioa_def paxos_asig_def Let_def split!:if_splits)
-  subgoal proof (cases "id (lstate s a) = leader (local_state.ballot (lstate s a))")
+  subgoal proof (cases "id (lstate s a) = leader (acc.ballot (lstate s a))")
     case False
     with prems(3,5,6) have "update_hist s h act s' = h" apply (simp add:update_hist_def receive_fwd_def)
     thm prems
@@ -421,7 +474,7 @@ definition propCmd2 where "propCmd2 s \<equiv> {v . \<exists> a \<in> as .
 
 definition fwd_sim where "fwd_sim s \<equiv> {t . 
   ampr1_state.propCmd t = propCmd s
-  \<and> ballot t = (\<lambda> a . local_state.ballot (lstate s a))
+  \<and> ballot t = (\<lambda> a . acc.ballot (lstate s a))
   \<and> (\<forall> i b v . suggestion t i b = None \<longleftrightarrow> (\<forall> a . Packet a (Phase2a i b v) \<notin> network s))
   \<and> (\<forall> i b v . suggestion t i b = Some v \<longleftrightarrow> (\<forall> a . a \<noteq> leader b \<longrightarrow> Packet a (Phase2a i b v) \<in> network s))
   \<and> (\<forall> i b v a . vote t i a b = None \<longleftrightarrow> (\<forall> a2 . Packet a2 (Phase2b a i b v) \<notin> network s))
@@ -450,17 +503,17 @@ lemma "is_forward_sim fwd_sim ampr3_ioa ampr1_ioa"
           filter_act_def ampr1_ioa_def r1.ioa_def paxos_asig_def Let_def is_trans_def 
           r1.trans_def split!:if_splits)
        apply simp
-      subgoal proof (cases "leader (local_state.ballot (lstate s a)) = local_state.id (lstate s a)")
+      subgoal proof (cases "leader (acc.ballot (lstate s a)) = acc.id (lstate s a)")
         case False
         with prems(1,4) show ?thesis by (simp add:propose_def send_all_def fwd_sim_def propCmd_def)
       next
         case True thm prems
-        have 1:"\<And> a . local_state.ballot (lstate t a) = ballot s' a" using prems(1,4) True 
+        have 1:"\<And> a . acc.ballot (lstate t a) = ballot s' a" using prems(1,4) True 
           by (simp add:do_2a_def propose_def send_all_def fwd_sim_def Let_def propCmd_def)
-        have 2:"network t = network s \<union> {Packet a2 (Phase2a (next_inst (lstate s a)) (local_state.ballot (lstate s a)) v) 
+        have 2:"network t = network s \<union> {Packet a2 (Phase2a (next_inst (lstate s a)) (acc.ballot (lstate s a)) v) 
             | a2 . a2 \<noteq> a \<and> a2 \<in> acceptors (lstate s a)}"
           using prems(4,2) True
-          by (fastforce simp add:do_2a_def propose_def send_all_def fwd_sim_def propCmd_def Let_def inv1_def)
+          by (fastforce simp add:do_2a_def propose_def send_all_def fwd_sim_def propCmd_def Let_def inv1_def) oops
         show ?thesis using 1 2 prems(1,2) apply (auto simp add:sim_defs inv1_def split!:msg.splits packet.splits)
               apply (metis ref_proof_3.axioms(2) ref_proof_3_axioms ref_proof_3_axioms_def)
              apply meson defer
